src/high/resources/preorders.v
@@ -4,94 +4,62 @@
    The preorders are stored in encoded format in the RA because the preorder may
    be over an arbitrary type. *)
 
-From iris.algebra Require Import auth gmap.
+From iris.algebra Require Import auth gmap gmap_view.
 From iris.base_logic.lib Require Import own.
 From iris.heap_lang Require Export locations.
 From iris.proofmode Require Import proofmode.
 
 From self Require Import extra encode_relation.
+From self.algebra Require Import ghost_map.
 
 (* Resource algebra that stores the encoded preorder for each location. *)
 Definition relationO := leibnizO (positive → positive → Prop).
-Definition preordersR := authR (gmapUR loc (agreeR relationO)).
+(* Definition preordersG Σ := ghost_mapG Σ loc (relation2 positive). *)
 
 Section preorders.
-  Context `{inG Σ preordersR}.
+  (* Context `{preordersG Σ}. *)
+  Context `{ghost_mapG Σ loc (relation2 positive)}.
   Context `{Countable A}.
 
   Implicit Type (preorders : gmap loc (relation2 positive)).
 
-  Definition map_to_agree preorders : gmapUR _ (agreeR relationO) :=
-    to_agree <$> preorders.
-
   Definition own_all_preorders γ preorders :=
-    own γ (● (map_to_agree preorders)).
-
-  (* Definition own_all_preorders preorders := *)
-  (*   own_all_preorders_gname preorders_name preorders. *)
+    ghost_map_auth γ (DfracOwn 1) preorders.
 
   Definition own_know_preorder_loc γ ℓ (preorder : relation2 A) : iProp Σ :=
-    own γ (◯ ({[ ℓ := to_agree (encode_relation preorder) ]})).
-
-  (* Global Instance persistent_know_preorder_loc ℓ preorder : *)
-  (*   Persistent (know_preorder_loc ℓ preorder). *)
-  (* Proof. apply _. Qed. *)
+    ℓ ↪[γ]□ encode_relation preorder.
 
   Lemma own_all_preorders_gname_alloc (preorders : gmap loc (relation2 positive)) :
-    ⊢ |==> ∃ γ, own_all_preorders γ preorders ∗
-                own γ (◯ ((to_agree <$> preorders) : gmapUR _ (agreeR relationO))).
-  Proof.
-    setoid_rewrite <- own_op.
-    iApply own_alloc.
-    apply auth_both_valid_discrete. split; first done.
-    rewrite /map_to_agree.
-    apply (valid_to_agree_fmap (B := relationO) preorders).
-  Qed.
+    ⊢ |==> ∃ γ,
+      own_all_preorders γ preorders ∗ ([∗ map] ℓ ↦ p ∈ preorders, ℓ ↪[γ]□ p).
+  Proof. by iMod (ghost_map_alloc_persistent). Qed.
 
-  Lemma own_all_preorders_persist γ preorders :
-    own_all_preorders γ preorders ==∗
-    own γ (●□ ((to_agree <$> preorders) : gmapUR _ (agreeR relationO))).
-  Proof. iApply own_update. apply auth_update_auth_persist. Qed.
-
-  Lemma auth_valid_to_agree_singleton_l {B}
-        dq (m : gmap loc (leibnizO B)) e (ℓ : loc) :
-    ✓ (●{dq} (to_agree <$> m : gmapUR _ (agreeR _)) ⋅
-       ◯ {[ℓ := to_agree e]}) →
-    m !! ℓ = Some e.
-  Proof.
-    intros [_ [incl _]]%auth_both_dfrac_valid_discrete.
-    move: incl.
-    rewrite singleton_included_l.
-    intros [y [eq incl]].
-    move: incl.
-    rewrite lookup_fmap in eq.
-    apply Some_equiv_eq in eq.
-    destruct eq as [y' [look' eq]].
-    rewrite -eq.
-    rewrite <- look'.
-    rewrite option_included_total.
-    intros [|(? & ? & [= ?] & [= ?] & incl)]; first done.
-    destruct (m !! ℓ) as [encOrder|]; last done.
-    simpl in *.
-    simplify_eq.
-    setoid_rewrite to_agree_included in incl.
-    f_equiv.
-    apply leibniz_equiv.
-    done.
-  Qed.
-
-  Lemma own_all_preorders_singleton_frag dq γ (ℓ : loc) preorders
-        (preorder : relation A) :
-    own γ (●{dq} (map_to_agree preorders)) -∗
-    own γ (◯ ({[ ℓ := to_agree (encode_relation preorder)]})) -∗
-    ⌜preorders !! ℓ = Some (encode_relation preorder)⌝.
-  Proof.
-    iIntros "auth frag".
-    iDestruct (own_valid_2 with "auth frag") as %V.
-    iPureIntro.
-    eapply auth_valid_to_agree_singleton_l.
-    apply V.
-  Qed.
+  (* Lemma auth_valid_to_agree_singleton_l {B} *)
+  (*       dq (m : gmap loc (leibnizO B)) e (ℓ : loc) : *)
+  (*   ✓ (●{dq} (to_agree <$> m : gmapUR _ (agreeR _)) ⋅ *)
+  (*      ◯ {[ℓ := to_agree e]}) → *)
+  (*   m !! ℓ = Some e. *)
+  (* Proof. *)
+  (*   intros [_ [incl _]]%auth_both_dfrac_valid_discrete. *)
+  (*   move: incl. *)
+  (*   rewrite singleton_included_l. *)
+  (*   intros [y [eq incl]]. *)
+  (*   move: incl. *)
+  (*   rewrite lookup_fmap in eq. *)
+  (*   apply Some_equiv_eq in eq. *)
+  (*   destruct eq as [y' [look' eq]]. *)
+  (*   rewrite -eq. *)
+  (*   rewrite <- look'. *)
+  (*   rewrite option_included_total. *)
+  (*   intros [|(? & ? & [= ?] & [= ?] & incl)]; first done. *)
+  (*   destruct (m !! ℓ) as [encOrder|]; last done. *)
+  (*   simpl in *. *)
+  (*   simplify_eq. *)
+  (*   setoid_rewrite to_agree_included in incl. *)
+  (*   f_equiv. *)
+  (*   apply leibniz_equiv. *)
+  (*   done. *)
+  (* Qed. *)
 
   Lemma orders_lookup γ ℓ order1 order2 (orders : gmap loc (relation2 positive)) :
     orders !! ℓ = Some order1 →
@@ -100,22 +68,8 @@ Section preorders.
     ⌜order1 = encode_relation order2⌝.
   Proof.
     iIntros (look) "auth frag".
-    iDestruct (own_all_preorders_singleton_frag with "auth frag")
-      as %look'.
-    simplify_eq. done.
-  Qed.
-
-  Lemma orders_frag_lookup γ preorders (ℓ : loc) order :
-    preorders !! ℓ = Some order →
-    own γ (◯ (map_to_agree preorders)) -∗
-    own γ (◯ ({[ ℓ := to_agree order ]} : gmapUR _ (agreeR relationO))).
-  Proof.
-    intros look. f_equiv. simpl.
-    apply auth_frag_mono.
-    rewrite singleton_included_l.
-    eexists _.
-    rewrite lookup_fmap look.
-    naive_solver.
+    iDestruct (ghost_map_lookup with "auth frag") as "%".
+    iPureIntro. congruence.
   Qed.
 
 End preorders.
